Matroid/Intersection.lean
@@ -1,0 +1,348 @@
+
+import Matroid.Constructions.DirectSum
+import Matroid.Minor.Rank
+
+-- /- Here we prove Edmonds' matroid intersection theorem: given two matroids `M₁` and `M₂` on `α`, the
+--   largest set that is independent in both matroids has size equal to the min of `M₁.r X + M₂.r Xᶜ`,
+--   taken over all `X ⊆ E`. We also derive Rado's theorem as a corollary. -/
+
+-- open_locale classical
+
+-- open matroid set
+
+-- variables {E : Type*} [finite E] {M M₁ M₂ : matroid E} {I A : set E}
+
+-- section intersection
+open Set
+
+namespace Matroid
+
+variable {α : Type*} {M M₁ M₂ : Matroid α} {A I X E : Set α}
+
+lemma Indep.ncard_le_r_add_r [FiniteRk M₁] [FiniteRk M₂] (hI₁ : M₁.Indep I) (hI₂ : M₂.Indep I)
+    (A : Set α) : I.ncard ≤ M₁.r A + M₂.r (M₂.E \ A) := by
+  rw [← ncard_inter_add_ncard_diff_eq_ncard I A hI₂.finite, ← (hI₁.inter_right A).r,
+    ← (hI₂.diff A).r]
+  exact add_le_add (M₁.r_mono inter_subset_right)
+    (M₂.r_mono (diff_subset_diff_left hI₂.subset_ground))
+
+lemma Indep.basis'_basis'_of_ncard_eq [FiniteRk M₁] [FiniteRk M₂] (hI₁ : M₁.Indep I)
+    (hI₂ : M₂.Indep I) (h : M₁.r A + M₂.r (M₂.E \ A) ≤ I.ncard) :
+    M₁.Basis' (I ∩ A) A ∧ M₂.Basis' (I \ A) (M₂.E \ A) := by
+  rw [basis'_iff_indep_encard_eq_of_finite (hI₁.finite.subset inter_subset_left),
+    and_iff_right inter_subset_right, and_iff_right (hI₁.inter_right A),
+    basis'_iff_indep_encard_eq_of_finite (hI₁.finite.diff _), and_iff_right (hI₂.diff A),
+    and_iff_right (diff_subset_diff_left hI₂.subset_ground), ← (hI₂.diff A).er,
+    er_eq_er_iff, ← (hI₁.inter_right A).er, er_eq_er_iff]
+
+  rw [← ncard_inter_add_ncard_diff_eq_ncard I A hI₂.finite, ← (hI₁.inter_right A).r,
+    ← (hI₂.diff A).r] at h
+  constructor <;>
+  linarith [M₁.r_mono (show I ∩ A ⊆ A from inter_subset_right),
+    M₂.r_mono (show I \ A ⊆ M₂.E \ A from diff_subset_diff_left hI₂.subset_ground)]
+
+lemma exists_common_ind' (M₁ M₂ : Matroid α) [M₁.Finite] [M₂.Finite] :
+    ∃ I X, M₁.Indep I ∧ M₂.Indep I ∧ I.ncard = M₁.r X + M₂.r Xᶜ := by
+
+  obtain (h | ⟨e, he₁, he₂⟩) := em' <| ∃ e, M₁.Nonloop e ∧ M₂.Nonloop e
+  · refine ⟨∅, (M₂.E \ M₁.E) ∪ M₁.cl ∅, ?_⟩
+    rw [M₂.r_eq_r_inter_ground, inter_comm, ← diff_eq, ← diff_diff, r_eq_r_inter_ground,
+      union_inter_distrib_right]
+    suffices 0 = M₂.r ((M₂.E ∩ M₁.E) \ M₁.cl ∅) by simpa [← r_eq_r_inter_ground]
+    rw [eq_comm, r_eq_zero_iff (diff_subset.trans inter_subset_left), diff_subset_iff, inter_comm]
+    simp_rw [subset_def, mem_union, ← loop_iff_mem_cl_empty]
+    by_contra! hcon
+    obtain ⟨x, ⟨h₁, h₂⟩, h'⟩ := hcon
+    exact h ⟨x, (not_loop_iff h₁).1 h'.1, (not_loop_iff h₂).1 h'.2⟩
+
+  have : (M₁ ／ e).E.ncard < M₁.E.ncard :=
+    ncard_lt_ncard (by simpa using he₁.mem_ground) M₁.ground_finite
+  have : (M₁ ＼ e).E.ncard < M₁.E.ncard :=
+    ncard_lt_ncard (by simpa using he₁.mem_ground) M₁.ground_finite
+
+  obtain ⟨Id, Xd, hId₁, hId₂, hId⟩ := exists_common_ind' (M₁ ＼ e) (M₂ ＼ e)
+  obtain ⟨Ic, Xc, hIc₁, hIc₂, hIc⟩ := exists_common_ind' (M₁ ／ e) (M₂ ／ e)
+
+
+termination_by M₁.E.ncard
+
+    -- simp only [empty_indep, ncard_empty, sdiff_sdiff_right_self, inf_eq_inter, true_and]
+
+    -- simp only [empty_indep, ncard_empty, true_and]
+    -- rw [r_eq_r_inter_ground, union_inter_distrib_right, diff_inter_self, union_empty,
+    --   ← r_eq_r_inter_ground, r_loops, zero_add, r_eq_r_inter_ground, compl_union, inter_assoc,
+    --   diff_eq, compl_inter, compl_compl, union_inter_distrib_right, compl_inter_self, empty_union,
+    --   eq_comm, ← inter_assoc, r_eq_zero_iff inter_subset_right, inter_assoc, ← diff_eq_compl_inter,
+    --   diff_subset_iff]
+    -- sorry
+
+
+
+
+
+  --   by_cases hloop : ∀ e ∈ M₁.E, M₁.Loop e ∨ M₂.Loop e
+  -- · suffices 0 = M₂.r (M₂.E \ M₁.cl ∅) from ⟨∅, M₁.cl ∅, cl_subset_ground _ _, by simpa⟩
+  --   rw [eq_comm, r_eq_zero_iff diff_subset, diff_subset_iff, ← hE]
+  --   simpa [subset_def]
+  -- push_neg at hloop
+  -- obtain ⟨e, he, he₁, he₂⟩ := hloop
+  -- rw [not_loop_iff] at he₁ he₂
+
+  -- have : (M₁ ／ e).E.ncard < M₁.E.ncard := ncard_lt_ncard (by simpa) M₁.ground_finite
+  -- have : (M₁ ＼ e).E.ncard < M₁.E.ncard := ncard_lt_ncard (by simpa) M₁.ground_finite
+
+lemma exists_common_ind (M₁ M₂ : Matroid α) [M₁.Finite] (hE : M₁.E = M₂.E) :
+    ∃ I X, X ⊆ M₁.E ∧ M₁.Indep I ∧ M₂.Indep I ∧ I.ncard = M₁.r X + M₂.r (M₂.E \ X) := by
+  have _ : M₂.Finite := ⟨hE.symm ▸ M₁.ground_finite⟩
+  by_cases hloop : ∀ e ∈ M₁.E, M₁.Loop e ∨ M₂.Loop e
+  · suffices 0 = M₂.r (M₂.E \ M₁.cl ∅) from ⟨∅, M₁.cl ∅, cl_subset_ground _ _, by simpa⟩
+    rw [eq_comm, r_eq_zero_iff diff_subset, diff_subset_iff, ← hE]
+    simpa [subset_def]
+  push_neg at hloop
+  obtain ⟨e, he, he₁, he₂⟩ := hloop
+  rw [not_loop_iff] at he₁ he₂
+
+  have : (M₁ ／ e).E.ncard < M₁.E.ncard := ncard_lt_ncard (by simpa) M₁.ground_finite
+  have : (M₁ ＼ e).E.ncard < M₁.E.ncard := ncard_lt_ncard (by simpa) M₁.ground_finite
+
+  obtain ⟨Id, Xd, hXd, hId₁, hId₂, hId⟩ := exists_common_ind (M₁ ＼ e) (M₂ ＼ e) (by simp [hE])
+  obtain ⟨Ic, Xc, hXc, hIc₁, hIc₂, hIc⟩ := exists_common_ind (M₁ ／ e) (M₂ ／ e) (by simp [hE])
+
+  rw [he₁.contract_indep_iff] at hIc₁
+  rw [he₂.contract_indep_iff] at hIc₂
+
+  simp only [contract_elem, contract_ground, deleteElem, delete_ground,
+    subset_diff_singleton_iff] at hXc hXd
+
+  by_contra! hcon
+  replace hcon :=
+    show ∀ I X, X ⊆ M₁.E → M₁.Indep I → M₂.Indep I → I.ncard + 1 ≤ M₁.r X + M₂.r (M₂.E \ X) from
+    fun I X hX h h' ↦ Nat.add_one_le_iff.2 <| (h.ncard_le_r_add_r h' X).lt_of_ne <| hcon I X hX h h'
+
+  have hcond := hcon Id (Xc ∩ Xd) (inter_subset_left.trans hXc.1) hId₁.of_delete hId₂.of_delete
+
+  replace hcon := hcon (insert e Ic) (insert e (Xc ∪ Xd))
+    (insert_subset he₁.mem_ground (union_subset hXc.1 hXd.1)) hIc₁.2 hIc₂.2
+  rw [ncard_insert_of_not_mem hIc₁.1 (hIc₁.2.subset (subset_insert _ _)).finite,
+    ← insert_union] at hcon
+
+  have hsm := M₁.r_submod (insert e Xc) Xd
+  rw [insert_inter_of_not_mem hXd.2] at hsm
+
+  have hsm2 := M₂.r_submod (M₂.E \ Xc) ((M₂.E \ insert e Xd))
+  simp_rw [diff_eq, ← inter_inter_distrib_left, ← inter_union_distrib_left, ← compl_inter,
+    ← compl_union, union_insert, ← insert_union, inter_comm Xc, insert_inter_of_not_mem hXc.2,
+    inter_comm Xd, ← diff_eq] at hsm2
+
+  zify at hcon hcond hId hIc hsm hsm2
+
+  rw [he₂.contract_r_cast_int_eq, he₁.contract_r_cast_int_eq, contract_elem, contract_ground,
+    diff_diff_comm, insert_diff_singleton,
+      insert_eq_of_mem (show e ∈ M₂.E \ Xc from ⟨he₂.mem_ground, hXc.2⟩)] at hIc
+  rw [delete_elem_r_eq _ hXd.2, delete_elem_r_eq _ (by simp), deleteElem, delete_ground,
+    diff_diff_comm, diff_diff, union_singleton] at hId
+
+  linarith
+
+termination_by M₁.E.ncard
+
+/-- We can choose a minimizing pair `I,X` where `X` is a flat of `M₁` -/
+lemma exists_common_ind_with_flat_left (M₁ M₂ : Matroid α) [M₁.Finite] (hE : M₁.E = M₂.E) :
+  ∃ I X, M₁.Indep I ∧ M₂.Indep I ∧ I.ncard = M₁.r X + M₂.r (M₂.E \ X) ∧ M₁.flat X :=
+
+-- /-- The hard direction of matroid intersection : existence -/
+-- lemma exists_common_ind (M₁ M₂ : matroid E) :
+--   ∃ I X, M₁.indep I ∧ M₂.indep I ∧ I.ncard = M₁.r X + M₂.r Xᶜ :=
+-- begin
+--   -- Suppose not. Then we get strict inequality for all choices of I, X.
+--   by_contra' hcon,
+--   have hcon' : ∀ I X, M₁.indep I → M₂.indep I → I.ncard < M₁.r X + M₂.r Xᶜ, from
+--     λ I X hI₁ hI₂, lt_of_le_of_ne (common_ind_le_r_add_r_compl hI₁ hI₂ X) (hcon I X hI₁ hI₂),
+
+--   -- Construct a minimal counterexample (wrt the number of nonloops of `M₁`)
+--   obtain ⟨M,hM,hpmin⟩ := (to_finite _ : {M | ∃ M', _}.finite).exists_minimal_wrt
+--     (ncard ∘ matroid.nonloops) ⟨M₁, ⟨M₂, hcon'⟩⟩,
+
+--   clear hcon hcon' M₁ M₂,
+--   obtain ⟨M₁,M₂,hcon⟩ := ⟨M,hM⟩,
+
+--   -- There is a common nonloop of `M₁` and `M₂`, otherwise the result is easy
+--   have hne : ∃ e, M₁.nonloop e ∧ M₂.nonloop e,
+--   { simp_rw [←not_loop_iff], by_contra' he,
+--     simp_rw [loop_iff_mem_cl_empty, ←mem_compl_iff, ←subset_def] at he,
+--     specialize hcon ∅ (M₁.cl ∅) M₁.empty_indep M₂.empty_indep,
+--     rw [ncard_empty, r_cl, r_empty, zero_add] at hcon,
+--     exact (hcon.trans_le (M₂.r_mono he)).ne (by rw [r_cl, r_empty])},
+
+--   obtain ⟨e, he₁,he₂⟩ := hne,
+
+--   -- Projecting/loopifying `e` gives non-counterexamples (by minimality), so there exist pairs
+--   -- with equality in these minors.
+--   have hd' := ncard_lt_ncard (strict_pminor_of_loopify_nonloop he₁).nonloops_ssubset_nonloops,
+--   refine hd'.ne.symm (hpmin (M₁ ⟍ e) ⟨M₂ ⟍ e,_⟩ hd'.le),
+--   by_contra' hd,
+--   obtain ⟨Id,Xd, hId₁, hId₂, hId⟩ := hd,
+
+--   have hc' := ncard_lt_ncard (strict_pminor_of_project_nonloop he₁).nonloops_ssubset_nonloops,
+--   refine hc'.ne.symm (hpmin (M₁ ⟋ e) ⟨M₂ ⟋ e,_⟩ hc'.le),
+--   by_contra' hc,
+--   obtain ⟨Ic,Xc, hIc₁, hIc₂, hIc⟩ := hc,
+
+--   -- Use these pairs to get rank lower bounds ...
+--   have hi := (hId.trans_lt (hcon _ ((Xc ∩ Xd) \ {e}) hId₁.of_loopify hId₂.of_loopify)),
+
+--   have hic : (Xc ∩ Xd \ {e})ᶜ = (insert e (Xcᶜ ∪ Xdᶜ)),
+--   { apply compl_injective,
+--     simp_rw [←union_singleton, compl_union, compl_compl, diff_eq_compl_inter, inter_comm {e}ᶜ]},
+
+--   simp_rw [loopify_elem, loopify.r_eq, hic] at hi,
+--   zify at hIc hId hcon,
+
+--   have hu := hcon (insert e Ic) (insert e (Xc ∪ Xd))
+--     (by rwa ← he₁.indep_project_iff (not_mem_of_indep_project_singleton hIc₁))
+--     (by rwa ← he₂.indep_project_iff (not_mem_of_indep_project_singleton hIc₁)),
+
+--   have huc : (insert e (Xc ∪ Xd))ᶜ = Xcᶜ ∩ Xdᶜ \ {e},
+--   { apply compl_injective,
+--     simp_rw [diff_eq_compl_inter, compl_inter, compl_compl, singleton_union]},
+
+--   simp_rw [ncard_insert_of_not_mem (not_mem_of_indep_project_singleton hIc₁),
+--     nat.cast_add, nat.cast_one, huc] at hu,
+
+--   rw [he₁.cast_r_project_eq, he₂.cast_r_project_eq] at hIc,
+
+--   -- ... and contradict them with submodularity bounds.
+--   have sm1 := M₁.r_submod (insert e Xc) (Xd \ {e}),
+--   have sm2 := M₂.r_submod (insert e Xcᶜ) (Xdᶜ \ {e}),
+
+--   rw [insert_union, insert_union_distrib, insert_diff_singleton, ←insert_union_distrib,
+--     insert_inter_of_not_mem (not_mem_diff_singleton _ _), ←inter_diff_assoc] at sm1 sm2,
+
+--   linarith,
+-- end
+
+-- /-- We can choose a minimizing pair `I,X` where `X` is a flat of `M₁` -/
+-- lemma exists_common_ind_with_flat_left (M₁ M₂ : matroid E) :
+--   ∃ I X, M₁.indep I ∧ M₂.indep I ∧ I.ncard = M₁.r X + M₂.r Xᶜ ∧ M₁.flat X :=
+-- begin
+--   obtain ⟨I,X₀, h₀⟩ := exists_common_ind M₁ M₂,
+--   rw [←M₁.r_cl X₀] at h₀,
+--   refine ⟨I,M₁.cl X₀,h₀.1, h₀.2.1, le_antisymm _ _, M₁.flat_of_cl _⟩,
+--   { apply common_ind_le_r_add_r_compl h₀.1 h₀.2.1 },
+--   rw h₀.2.2,
+--   simp only [add_le_add_iff_left],
+--   exact M₂.r_mono (compl_subset_compl.mpr (subset_cl _ _)),
+-- end
+
+-- lemma exists_common_ind_with_flat_right (M₁ M₂ : matroid E) :
+--   ∃ I X, M₁.indep I ∧ M₂.indep I ∧ I.ncard = M₁.r X + M₂.r Xᶜ ∧ M₂.flat Xᶜ :=
+-- begin
+--   obtain ⟨I,X₀,h₀,h₁,hX₀,hF⟩ := exists_common_ind_with_flat_left M₂ M₁,
+--   exact ⟨I, X₀ᶜ,h₁,h₀,by rwa [add_comm, compl_compl],by rwa compl_compl⟩,
+-- end
+
+-- /-- The cardinality of a largest common independent set of matroids `M₁,M₂`.
+--   Is `find_greatest` really the right way to define this?  -/
+-- noncomputable def max_common_ind (M₁ M₂ : matroid E) :=
+-- nat.find_greatest (λ n, ∃ I, M₁.indep I ∧ M₂.indep I ∧ I.ncard = n) ((univ : set E).ncard)
+
+-- lemma max_common_ind_eq_iff (M₁ M₂ : matroid E) {n : ℕ} :
+--   max_common_ind M₁ M₂ = n ↔ (∃ I, M₁.indep I ∧ M₂.indep I ∧ n ≤ I.ncard) ∧
+--     (∀ I, M₁.indep I → M₂.indep I → I.ncard ≤ n)  :=
+-- begin
+--   rw [max_common_ind, nat.find_greatest_eq_iff],
+--   obtain (rfl | n) := n,
+--   { simp only [nat.nat_zero_eq_zero, zero_le', ne.def, eq_self_iff_true, not_true, ncard_eq_zero,
+--     exists_eq_right_right, is_empty.forall_iff, not_exists, not_and, true_and, le_zero_iff,
+--     and_true],
+--     split,
+--     {
+--       refine λ h, ⟨⟨_, M₁.empty_indep, M₂.empty_indep⟩, λ I hI₁ hI₂, _⟩,
+--       suffices hcI : ¬(0 < I.ncard), by rwa [not_lt, le_zero_iff, ncard_eq_zero] at hcI,
+--       exact λ hcI, h hcI (ncard_mono (subset_univ _)) I hI₁ hI₂ rfl},
+--     refine λ h n hpos hn I hI₁ hI₂ hcard, _,
+--     rw [←hcard, h.2 I hI₁ hI₂] at hpos,
+--     simpa using hpos},
+
+--   simp only [ne.def, nat.succ_ne_zero, not_false_iff, forall_true_left, not_exists, not_and,
+--     nat.succ_eq_add_one],
+--   split,
+--   { rintro ⟨hn, ⟨I, hI₁, hI₂, hIcard⟩, h'⟩,
+--     refine ⟨⟨I, hI₁, hI₂, hIcard.symm.le⟩, λ J hJ₁ hJ₂, _⟩,
+--     by_contra' hJcard,
+--     exact h' hJcard (ncard_mono (subset_univ _)) J hJ₁ hJ₂ rfl},
+--   simp only [and_imp, forall_exists_index],
+--   refine λ I hI₁ hI₂ hIcard h, ⟨_,⟨I, hI₁,hI₂,_⟩ ,λ n' hn' hn'' J hJ₁ hJ₂ hJcard, _⟩,
+--   { rw ←(h I hI₁ hI₂).antisymm hIcard, exact ncard_mono (subset_univ _)},
+--   { rw ←(h I hI₁ hI₂).antisymm hIcard},
+--   subst hJcard,
+--   exact (h J hJ₁ hJ₂).not_lt hn',
+-- end
+
+-- theorem matroid_intersection_minmax (M₁ M₂ : matroid E) :
+--   max_common_ind M₁ M₂ = ⨅ X, M₁.r X + M₂.r Xᶜ :=
+-- begin
+--   rw [max_common_ind_eq_iff],
+--   obtain ⟨I, X, hI₁, hI₂, heq⟩ := exists_common_ind M₁ M₂,
+--   refine ⟨⟨I, hI₁, hI₂, (cinfi_le' _ _).trans_eq heq.symm⟩, λ J hJ₁ hJ₂, _ ⟩,
+--   exact (le_cinfi_iff (order_bot.bdd_below _)).mpr (common_ind_le_r_add_r_compl hJ₁ hJ₂),
+-- end
+
+-- end intersection
+
+-- section rado
+
+-- variables {ι : Type} [finite ι]
+
+-- lemma rado_necessary {f : E → ι} {x : ι → E} (hx : ∀ i, f (x i) = i) (h_ind : M.indep (range x))
+-- (S : set ι) :
+--   S.ncard ≤ M.r (f ⁻¹' S) :=
+-- begin
+--   have hS := (h_ind.subset (image_subset_range x S)).r,
+--   rw [ncard_image_of_injective _ (λ i j hij, by rw [←hx i, hij, hx j] : x.injective)] at hS,
+--   rw ←hS,
+--   refine M.r_mono _,
+--   rintro f ⟨i, hi, rfl⟩,
+--   rwa [mem_preimage, hx],
+-- end
+
+-- lemma rado_sufficient (f : E → ι) (h : ∀ (S : set ι), S.ncard ≤ M.r (f ⁻¹' S)) :
+--   ∃ (x : ι → E), (∀ i, f (x i) = i) ∧ M.indep (range x) :=
+-- begin
+--   set M' := partition_matroid_on f 1 with hM',
+--   obtain ⟨I, X, hI₁, hI₂, hIX, hF⟩ := exists_common_ind_with_flat_right M M',
+--   obtain ⟨hIb₁,hIb₂⟩ := common_ind_eq_spec hI₁ hI₂ hIX.symm.le,
+
+--   have h_inj : inj_on f I,
+--   { refine λ a ha b hb hab, by_contra (λ (hne : a ≠ b), _),
+--     have hcard := (partition_matroid_on_indep_iff.mp hI₂) (f a),
+--     rw [pi.one_apply, ncard_le_one_iff] at hcard,
+--     exact hne (hcard ⟨ha, (by simp)⟩ ⟨hb, by simp [hab]⟩)},
+
+--   have hXc := (h (f '' Xᶜ)ᶜ).trans (M.r_mono _ : _ ≤ M.r X), swap,
+--   { simp only [preimage_subset_iff, mem_compl_iff, mem_image, not_exists, not_and, not_imp_not],
+--     exact λ a h, h _ rfl},
+
+--   simp only [partition_matroid_on_one_r_eq, pi.one_apply] at hIX,
+--   have hineq := (add_le_add_right hXc _).trans_eq hIX.symm,
+--   rw [add_comm, ncard_add_ncard_compl, ←ncard_univ, ←ncard_image_of_inj_on h_inj] at hineq,
+--   have himage := eq_of_subset_of_ncard_le (subset_univ _) hineq,
+
+--   have hinv : ∀ i, ∃ e ∈ I, f e = i,
+--   { simp_rw [←mem_image_iff_bex, himage], exact mem_univ},
+
+--   choose x hx using hinv,
+--   refine ⟨x, λi, (hx i).2, hI₁.subset _⟩,
+--   rintro e ⟨i,hi,rfl⟩,
+--   exact (hx i).1,
+-- end
+
+-- /-- Rado's theorem: Given a partition `f : E → ι` of the ground set `E` of a matroid `M`, there is a
+--   transversal of `f` that is independent in `M` if and only if the rank of the preimage of every set
+--   `S` in `ι` is at least its cardinality. -/
+-- theorem rado_iff {M : matroid E} {f : E → ι} :
+--   (∃ (x : ι → E), (∀ i, f (x i) = i) ∧ M.indep (range x)) ↔ ∀ S, ncard S ≤ M.r (f ⁻¹' S) :=
+-- ⟨λ h S, exists.elim h (λ x hx, rado_necessary hx.1 hx.2 _) , rado_sufficient _⟩
+
+
+-- end rado
