Matroid/Rank.lean
@@ -20,12 +20,12 @@ noncomputable def erk (M : Matroid α) : ℕ∞ :=
 /-- The rank `er X` of a set `X` is the cardinality of one of its bases -/
 noncomputable def er (M : Matroid α) (X : Set α) : ℕ∞ := (M ↾ X).erk
 
-theorem erk_eq_er_ground (M : Matroid α) : M.erk = M.er M.E := by
+lemma erk_eq_er_ground (M : Matroid α) : M.erk = M.er M.E := by
   rw [er, restrict_ground_eq_self]
 
-@[simp] theorem erk_restrict (M : Matroid α) (X : Set α) : (M ↾ X).erk = M.er X := rfl
+@[simp] lemma erk_restrict (M : Matroid α) (X : Set α) : (M ↾ X).erk = M.er X := rfl
 
-theorem Basis'.encard (hI : M.Basis' I X) : I.encard = M.er X := by
+lemma Basis'.encard (hI : M.Basis' I X) : I.encard = M.er X := by
   rw [er,erk]
   rw [← base_restrict_iff'] at hI
   have : _root_.Nonempty ↑{B | (M ↾ X).Base B} := ⟨I, hI⟩
@@ -33,113 +33,113 @@ theorem Basis'.encard (hI : M.Basis' I X) : I.encard = M.er X := by
   simp only [mem_setOf_eq, Subtype.forall]
   exact fun B' hB' ↦ hB'.card_eq_card_of_base hI
 
-theorem Basis.encard (hI : M.Basis I X) : I.encard = M.er X :=
+lemma Basis.encard (hI : M.Basis I X) : I.encard = M.er X :=
   hI.basis'.encard
 
-theorem eq_er_iff (hX : X ⊆ M.E := by aesop_mat) :
+lemma eq_er_iff (hX : X ⊆ M.E := by aesop_mat) :
     M.er X = n ↔ ∃ I, M.Basis I X ∧ I.encard = n :=
   ⟨fun h ↦ (M.exists_basis X).elim (fun I hI ↦ ⟨I, hI, by rw [hI.encard, ← h]⟩),
     fun ⟨ I, hI, hIc⟩ ↦ by rw [← hI.encard, hIc]⟩
 
-theorem Indep.er (hI : M.Indep I) : M.er I = I.encard :=
+lemma Indep.er (hI : M.Indep I) : M.er I = I.encard :=
   (eq_er_iff hI.subset_ground).mpr ⟨I, hI.basis_self, rfl⟩
 
-theorem Basis'.er (hIX : M.Basis' I X) : M.er I = M.er X := by rw [← hIX.encard, hIX.indep.er]
+lemma Basis'.er (hIX : M.Basis' I X) : M.er I = M.er X := by rw [← hIX.encard, hIX.indep.er]
 
-theorem Basis.er (hIX : M.Basis I X) : M.er I = M.er X := by rw [← hIX.encard, hIX.indep.er]
+lemma Basis.er (hIX : M.Basis I X) : M.er I = M.er X := by rw [← hIX.encard, hIX.indep.er]
 
-theorem Basis'.er_eq_encard (hIX : M.Basis' I X) : M.er X = I.encard := by
+lemma Basis'.er_eq_encard (hIX : M.Basis' I X) : M.er X = I.encard := by
   rw [← hIX.er, hIX.indep.er]
 
-theorem Basis.er_eq_encard (hIX : M.Basis I X) : M.er X = I.encard := by
+lemma Basis.er_eq_encard (hIX : M.Basis I X) : M.er X = I.encard := by
   rw [← hIX.er, hIX.indep.er]
 
-theorem Base.er (hB : M.Base B) : M.er B = M.erk := by
+lemma Base.er (hB : M.Base B) : M.er B = M.erk := by
   rw [hB.indep.er, erk_eq_er_ground, hB.basis_ground.encard]
 
-theorem Base.encard (hB : M.Base B) : B.encard = M.erk := by
+lemma Base.encard (hB : M.Base B) : B.encard = M.erk := by
   rw [hB.basis_ground.encard, erk_eq_er_ground]
 
-@[simp] theorem er_inter_ground_eq (M : Matroid α) (X : Set α) : M.er (X ∩ M.E) = M.er X := by
+@[simp] lemma er_inter_ground_eq (M : Matroid α) (X : Set α) : M.er (X ∩ M.E) = M.er X := by
   obtain ⟨I, hI⟩ := M.exists_basis' X; rw [← hI.basis_inter_ground.encard, ← hI.encard]
 
--- theorem Iso.er_image_eq {α β : Type*} {M : Matroid α} {N : Matroid β} (e : Iso M N) (X : Set α)
+-- lemma Iso.er_image_eq {α β : Type*} {M : Matroid α} {N : Matroid β} (e : Iso M N) (X : Set α)
 --     (hX : X ⊆ M.E := by aesop_mat) : N.er (e '' X) = M.er X := by
 --   obtain ⟨I,hI⟩ := M.exists_basis X
 --   rw [hI.er_eq_encard, (e.on_basis hI).er_eq_encard,
 --     (e.injOn_ground.mono hI.indep.subset_ground).encard_image]
 
-@[simp] theorem er_univ_eq (M : Matroid α) : M.er univ = M.erk := by
+@[simp] lemma er_univ_eq (M : Matroid α) : M.er univ = M.erk := by
   rw [← er_inter_ground_eq, univ_inter, erk_eq_er_ground]
 
--- theorem Iso.erk_eq_erk {α β : Type*} {M : Matroid α} {N : Matroid β} (e : Iso M N) :
+-- lemma Iso.erk_eq_erk {α β : Type*} {M : Matroid α} {N : Matroid β} (e : Iso M N) :
 --     M.erk = N.erk := by
 --   rw [erk_eq_er_ground, ← e.er_image_eq M.E, e.image_ground, erk_eq_er_ground]
 
-@[simp] theorem er_empty (M : Matroid α) : M.er ∅ = 0 := by
+@[simp] lemma er_empty (M : Matroid α) : M.er ∅ = 0 := by
   rw [← M.empty_indep.basis_self.encard, encard_empty]
 
-@[simp] theorem er_cl_eq (M : Matroid α) (X : Set α) : M.er (M.cl X) = M.er X := by
+@[simp] lemma er_cl_eq (M : Matroid α) (X : Set α) : M.er (M.cl X) = M.er X := by
   rw [← cl_inter_ground, ← M.er_inter_ground_eq X]
   obtain ⟨I, hI⟩ := M.exists_basis (X ∩ M.E)
   rw [← hI.er, ← hI.cl_eq_cl, hI.indep.basis_cl.er]
 
-@[simp] theorem er_union_cl_right_eq (M : Matroid α) (X Y : Set α) :
+@[simp] lemma er_union_cl_right_eq (M : Matroid α) (X Y : Set α) :
     M.er (X ∪ M.cl Y) = M.er (X ∪ Y) :=
   by rw [← er_cl_eq, cl_union_cl_right_eq, er_cl_eq]
 
-@[simp] theorem er_union_cl_left_eq (M : Matroid α) (X Y : Set α) :
+@[simp] lemma er_union_cl_left_eq (M : Matroid α) (X Y : Set α) :
     M.er (M.cl X ∪ Y) = M.er (X ∪ Y) := by
   rw [← er_cl_eq, cl_union_cl_left_eq, er_cl_eq]
 
-@[simp] theorem er_insert_cl_eq (M : Matroid α) (e : α) (X : Set α) :
+@[simp] lemma er_insert_cl_eq (M : Matroid α) (e : α) (X : Set α) :
     M.er (insert e (M.cl X)) = M.er (insert e X) := by
   rw [← union_singleton, er_union_cl_left_eq, union_singleton]
 
-@[simp] theorem restrict_er_eq' (M : Matroid α) (R X : Set α) : (M ↾ R).er X = M.er (X ∩ R) := by
+@[simp] lemma restrict_er_eq' (M : Matroid α) (R X : Set α) : (M ↾ R).er X = M.er (X ∩ R) := by
   obtain ⟨I, hI⟩ := (M ↾ R).exists_basis' X
   rw [hI.er_eq_encard]
   rw [basis'_iff_basis_inter_ground, basis_restrict_iff', restrict_ground_eq] at hI
   rw [← er_inter_ground_eq, ← hI.1.er_eq_encard]
 
-@[simp] theorem restrict_er_eq (M : Matroid α) (h : X ⊆ R) : (M ↾ R).er X = M.er X := by
+@[simp] lemma restrict_er_eq (M : Matroid α) (h : X ⊆ R) : (M ↾ R).er X = M.er X := by
   rw [restrict_er_eq', inter_eq_self_of_subset_left h]
 
-theorem er_lt_top_of_finite (M : Matroid α) (hX : X.Finite) : M.er X < ⊤ := by
+lemma er_lt_top_of_finite (M : Matroid α) (hX : X.Finite) : M.er X < ⊤ := by
   obtain ⟨I, hI⟩ := M.exists_basis' X
   rw [hI.er_eq_encard, encard_lt_top_iff]
   exact hX.subset hI.subset
 
-theorem Basis'.er_eq_er_union (hIX : M.Basis' I X) (Y : Set α) : M.er (I ∪ Y) = M.er (X ∪ Y) := by
+lemma Basis'.er_eq_er_union (hIX : M.Basis' I X) (Y : Set α) : M.er (I ∪ Y) = M.er (X ∪ Y) := by
   rw [← er_union_cl_left_eq, hIX.cl_eq_cl, er_union_cl_left_eq]
 
-theorem Basis'.er_eq_er_insert (hIX : M.Basis' I X) (e : α) :
+lemma Basis'.er_eq_er_insert (hIX : M.Basis' I X) (e : α) :
     M.er (insert e I) = M.er (insert e X) := by
   rw [← union_singleton, hIX.er_eq_er_union, union_singleton]
 
-theorem Basis.er_eq_er_union (hIX : M.Basis I X) (Y : Set α) : M.er (I ∪ Y) = M.er (X ∪ Y) :=
+lemma Basis.er_eq_er_union (hIX : M.Basis I X) (Y : Set α) : M.er (I ∪ Y) = M.er (X ∪ Y) :=
   hIX.basis'.er_eq_er_union Y
 
-theorem Basis.er_eq_er_insert (hIX : M.Basis I X) (e : α) : M.er (insert e I) = M.er (insert e X) :=
+lemma Basis.er_eq_er_insert (hIX : M.Basis I X) (e : α) : M.er (insert e I) = M.er (insert e X) :=
   by rw [← union_singleton, hIX.er_eq_er_union, union_singleton]
 
-theorem er_le_encard (M : Matroid α) (X : Set α) : M.er X ≤ X.encard := by
+lemma er_le_encard (M : Matroid α) (X : Set α) : M.er X ≤ X.encard := by
   obtain ⟨I, hI⟩ := M.exists_basis' X; rw [hI.er_eq_encard]; exact encard_mono hI.subset
 
-theorem erk_le_encard_ground (M : Matroid α) : M.erk ≤ M.E.encard :=
+lemma erk_le_encard_ground (M : Matroid α) : M.erk ≤ M.E.encard :=
   M.erk_eq_er_ground.trans_le $ M.er_le_encard M.E
 
-theorem er_mono (M : Matroid α) : Monotone M.er := by
+lemma er_mono (M : Matroid α) : Monotone M.er := by
   rintro X Y (hXY : X ⊆ Y)
   obtain ⟨I, hI⟩ := M.exists_basis' X
   obtain ⟨J, hJ, hIJ⟩ := hI.indep.subset_basis'_of_subset (hI.subset.trans hXY)
   rw [hI.er_eq_encard, hJ.er_eq_encard]
   exact encard_mono hIJ
 
-theorem er_le_erk (M : Matroid α) (X : Set α) : M.er X ≤ M.erk := by
+lemma er_le_erk (M : Matroid α) (X : Set α) : M.er X ≤ M.erk := by
   rw [erk_eq_er_ground, ← er_inter_ground_eq]; exact M.er_mono inter_subset_right
 
-theorem le_er_iff : n ≤ M.er X ↔ ∃ I, I ⊆ X ∧ M.Indep I ∧ I.encard = n := by
+lemma le_er_iff : n ≤ M.er X ↔ ∃ I, I ⊆ X ∧ M.Indep I ∧ I.encard = n := by
   refine' ⟨fun h ↦ _, fun ⟨I, hIX, hI, hIc⟩ ↦ _⟩
   · obtain ⟨J, hJ⟩ := M.exists_basis' X
     rw [← hJ.encard] at h
@@ -148,20 +148,20 @@ theorem le_er_iff : n ≤ M.er X ↔ ∃ I, I ⊆ X ∧ M.Indep I ∧ I.encard =
   rw [← hIc, ← hI.er]
   exact M.er_mono hIX
 
-theorem er_le_iff : M.er X ≤ n ↔ ∀ {I}, I ⊆ X → M.Indep I → I.encard ≤ n := by
+lemma er_le_iff : M.er X ≤ n ↔ ∀ {I}, I ⊆ X → M.Indep I → I.encard ≤ n := by
   refine ⟨fun h I hIX hI ↦ (hI.er.symm.trans_le ((M.er_mono hIX).trans h)), fun h ↦ ?_⟩
   obtain ⟨I, hI⟩ := M.exists_basis' X
   rw [← hI.encard]
   exact h hI.subset hI.indep
 
-theorem Indep.encard_le_er_of_subset (hI : M.Indep I) (hIX : I ⊆ X) : I.encard ≤ M.er X := by
+lemma Indep.encard_le_er_of_subset (hI : M.Indep I) (hIX : I ⊆ X) : I.encard ≤ M.er X := by
   rw [← hI.er]; exact M.er_mono hIX
 
-theorem Indep.encard_le_erk (hI : M.Indep I) : I.encard ≤ M.erk := by
+lemma Indep.encard_le_erk (hI : M.Indep I) : I.encard ≤ M.erk := by
   rw [← hI.er, erk_eq_er_ground]; exact M.er_mono hI.subset_ground
 
 /-- The submodularity axiom for the extended rank function -/
-theorem er_inter_add_er_union_le_er_add_er (M : Matroid α) (X Y : Set α) :
+lemma er_inter_add_er_union_le_er_add_er (M : Matroid α) (X Y : Set α) :
     M.er (X ∩ Y) + M.er (X ∪ Y) ≤ M.er X + M.er Y := by
   obtain ⟨Ii, hIi⟩ := M.exists_basis' (X ∩ Y)
   obtain ⟨IX, hIX, hIX'⟩ :=
@@ -174,59 +174,59 @@ theorem er_inter_add_er_union_le_er_add_er (M : Matroid α) (X Y : Set α) :
 
 alias er_submod := er_inter_add_er_union_le_er_add_er
 
-theorem er_eq_er_of_subset_le (hXY : X ⊆ Y) (hYX : M.er Y ≤ M.er X) : M.er X = M.er Y :=
+lemma er_eq_er_of_subset_le (hXY : X ⊆ Y) (hYX : M.er Y ≤ M.er X) : M.er X = M.er Y :=
   (M.er_mono hXY).antisymm hYX
 
-theorem er_union_le_er_add_er (M : Matroid α) (X Y : Set α) : M.er (X ∪ Y) ≤ M.er X + M.er Y :=
+lemma er_union_le_er_add_er (M : Matroid α) (X Y : Set α) : M.er (X ∪ Y) ≤ M.er X + M.er Y :=
   le_add_self.trans (M.er_submod X Y)
 
-theorem er_eq_er_union_er_le_zero (X : Set α) (hY : M.er Y ≤ 0) : M.er (X ∪ Y) = M.er X :=
+lemma er_eq_er_union_er_le_zero (X : Set α) (hY : M.er Y ≤ 0) : M.er (X ∪ Y) = M.er X :=
   (((M.er_union_le_er_add_er X Y).trans (add_le_add_left hY _)).trans_eq (add_zero _)).antisymm
     (M.er_mono subset_union_left)
 
-theorem er_eq_er_diff_er_le_zero (X : Set α) (hY : M.er Y ≤ 0) : M.er (X \ Y) = M.er X := by
+lemma er_eq_er_diff_er_le_zero (X : Set α) (hY : M.er Y ≤ 0) : M.er (X \ Y) = M.er X := by
   rw [← er_eq_er_union_er_le_zero (X \ Y) hY, diff_union_self, er_eq_er_union_er_le_zero _ hY]
 
-theorem er_le_er_inter_add_er_diff (X Y : Set α) : M.er X ≤ M.er (X ∩ Y) + M.er (X \ Y) := by
+lemma er_le_er_inter_add_er_diff (X Y : Set α) : M.er X ≤ M.er (X ∩ Y) + M.er (X \ Y) := by
   nth_rw 1 [← inter_union_diff X Y]; apply er_union_le_er_add_er
 
-theorem er_le_er_add_er_diff (h : Y ⊆ X) : M.er X ≤ M.er Y + M.er (X \ Y) := by
+lemma er_le_er_add_er_diff (h : Y ⊆ X) : M.er X ≤ M.er Y + M.er (X \ Y) := by
   nth_rw 1 [← union_diff_cancel h]; apply er_union_le_er_add_er
 
-theorem indep_iff_er_eq_encard_of_finite (hI : I.Finite) : M.Indep I ↔ M.er I = I.encard := by
+lemma indep_iff_er_eq_encard_of_finite (hI : I.Finite) : M.Indep I ↔ M.er I = I.encard := by
   refine' ⟨fun h ↦ by rw [h.er], fun h ↦ _⟩
   obtain ⟨J, hJ⟩ := M.exists_basis' I
   rw [← hI.eq_of_subset_of_encard_le hJ.subset]
   · exact hJ.indep
   rw [← h, ← hJ.er_eq_encard]
 
-theorem indep_iff_er_eq_card [Matroid.Finite M] (hI : I ⊆ M.E := by aesop_mat) :
+lemma indep_iff_er_eq_card [Matroid.Finite M] (hI : I ⊆ M.E := by aesop_mat) :
     M.Indep I ↔ M.er I = I.encard :=
   indep_iff_er_eq_encard_of_finite (M.set_finite I)
 
-theorem er_singleton_le (M : Matroid α) (e : α) : M.er {e} ≤ 1 := by
+lemma er_singleton_le (M : Matroid α) (e : α) : M.er {e} ≤ 1 := by
   obtain ⟨J, hJ⟩ := M.exists_basis' {e}
   rw [hJ.er_eq_encard, ← encard_singleton e]
   exact encard_mono hJ.subset
 
-theorem er_lt_encard_of_dep_of_finite (h : X.Finite) (hX : M.Dep X) : M.er X < X.encard :=
+lemma er_lt_encard_of_dep_of_finite (h : X.Finite) (hX : M.Dep X) : M.er X < X.encard :=
   lt_of_le_of_ne (M.er_le_encard X) fun h' ↦
     ((indep_iff_er_eq_encard_of_finite h).mpr h').not_dep hX
 
-theorem er_lt_encard_iff_dep_of_finite (hX : X.Finite) (hXE : X ⊆ M.E := by aesop_mat) :
+lemma er_lt_encard_iff_dep_of_finite (hX : X.Finite) (hXE : X ⊆ M.E := by aesop_mat) :
     M.er X < X.encard ↔ M.Dep X := by
   refine' ⟨fun h ↦ _, fun h ↦ er_lt_encard_of_dep_of_finite hX h⟩
   rw [← not_indep_iff, indep_iff_er_eq_encard_of_finite hX]
   exact h.ne
 
-theorem er_lt_encard_of_dep [Matroid.Finite M] (hX : M.Dep X) : M.er X < X.encard :=
+lemma er_lt_encard_of_dep [Matroid.Finite M] (hX : M.Dep X) : M.er X < X.encard :=
   er_lt_encard_of_dep_of_finite (M.set_finite X hX.subset_ground) hX
 
-theorem r_lt_card_iff_dep [Matroid.Finite M] (hXE : X ⊆ M.E := by aesop_mat) :
+lemma r_lt_card_iff_dep [Matroid.Finite M] (hXE : X ⊆ M.E := by aesop_mat) :
     M.er X < X.encard ↔ M.Dep X :=
   er_lt_encard_iff_dep_of_finite (M.set_finite X)
 
-theorem basis'_iff_indep_encard_eq_of_finite (hIfin : I.Finite) :
+lemma basis'_iff_indep_encard_eq_of_finite (hIfin : I.Finite) :
     M.Basis' I X ↔ I ⊆ X ∧ M.Indep I ∧ I.encard = M.er X := by
   refine' ⟨fun h ↦ ⟨h.subset,h.indep, h.er_eq_encard.symm⟩, fun ⟨hIX, hI, hcard⟩  ↦ _⟩
   rw [basis'_iff_basis_inter_ground]
@@ -236,35 +236,35 @@ theorem basis'_iff_indep_encard_eq_of_finite (hIfin : I.Finite) :
     (by rw [hcard, ← hJ.er_eq_encard, er_inter_ground_eq ])
   exact hJ.subset_cl
 
-theorem basis_iff_indep_encard_eq_of_finite (hIfin : I.Finite) (hX : X ⊆ M.E := by aesop_mat) :
+lemma basis_iff_indep_encard_eq_of_finite (hIfin : I.Finite) (hX : X ⊆ M.E := by aesop_mat) :
     M.Basis I X ↔ I ⊆ X ∧ M.Indep I ∧ I.encard = M.er X := by
   rw [← basis'_iff_basis, basis'_iff_indep_encard_eq_of_finite hIfin]
 
-theorem Indep.basis_of_subset_of_er_le_of_finite (hI : M.Indep I) (hIX : I ⊆ X)
+lemma Indep.basis_of_subset_of_er_le_of_finite (hI : M.Indep I) (hIX : I ⊆ X)
     (h : M.er X ≤ M.er I) (hIfin : I.Finite) (hX : X ⊆ M.E := by aesop_mat) : M.Basis I X := by
   rw [basis_iff_indep_encard_eq_of_finite hIfin hX, and_iff_right hIX, and_iff_right hI,
      le_antisymm_iff, and_iff_left (h.trans hI.er.le), ← hI.er]
   exact M.er_mono hIX
 
-theorem er_insert_le_add_one (M : Matroid α) (e : α) (X : Set α) :
+lemma er_insert_le_add_one (M : Matroid α) (e : α) (X : Set α) :
     M.er (insert e X) ≤ M.er X + 1 := by
   rw [← union_singleton]
   exact (M.er_union_le_er_add_er _ _).trans (add_le_add_left (er_singleton_le _ _) _)
 
-theorem er_union_le_encard_add_er (M : Matroid α) (X Y : Set α) :
+lemma er_union_le_encard_add_er (M : Matroid α) (X Y : Set α) :
     M.er (X ∪ Y) ≤ X.encard + M.er Y :=
   (M.er_union_le_er_add_er X Y).trans (add_le_add_right (M.er_le_encard _) _)
 
-theorem er_union_le_er_add_encard (M : Matroid α) (X Y : Set α) :
+lemma er_union_le_er_add_encard (M : Matroid α) (X Y : Set α) :
     M.er (X ∪ Y) ≤ M.er X + Y.encard :=
   (M.er_union_le_er_add_er X Y).trans (add_le_add_left (M.er_le_encard _) _)
 
-theorem erk_le_encard_add_er_compl (M : Matroid α) (X : Set α) :
+lemma erk_le_encard_add_er_compl (M : Matroid α) (X : Set α) :
     M.erk ≤ X.encard + M.er (M.E \ X) :=
   le_trans (by rw [← er_inter_ground_eq, erk_eq_er_ground, union_diff_self,
     union_inter_cancel_right]) (M.er_union_le_encard_add_er X (M.E \ X))
 
-theorem er_insert_eq_add_one (M : Matroid α) (X : Set α) (he : e ∈ M.E \ M.cl X) :
+lemma er_insert_eq_add_one (M : Matroid α) (X : Set α) (he : e ∈ M.E \ M.cl X) :
     M.er (insert e X) = M.er X + 1 := by
   obtain ⟨I, hI⟩ := M.exists_basis' X
   rw [← hI.cl_eq_cl] at he
@@ -274,7 +274,7 @@ theorem er_insert_eq_add_one (M : Matroid α) (X : Set α) (he : e ∈ M.E \ M.c
   rw [hI.indep.insert_indep_iff]
   exact Or.inl he
 
-theorem er_augment (h : M.er X < M.er Z) : ∃ z ∈ Z \ X, M.er (insert z X) = M.er X + 1 := by
+lemma er_augment (h : M.er X < M.er Z) : ∃ z ∈ Z \ X, M.er (insert z X) = M.er X + 1 := by
   obtain ⟨I, hI⟩ := M.exists_basis' X
   obtain ⟨J, hJ, hIJ⟩ := hI.indep.subset_basis'_of_subset (hI.subset.trans subset_union_left)
   have hlt := h.trans_le (M.er_mono (subset_union_right (s := X)))
@@ -286,7 +286,7 @@ theorem er_augment (h : M.er X < M.er Z) : ∃ z ∈ Z \ X, M.er (insert z X) = 
   refine ⟨e, ⟨Or.elim (hJ.subset heJ) (False.elim ∘ heX) id, heX⟩, ?_⟩
   rw [← hI.er_eq_er_insert, hI.er_eq_encard, heIi.er, encard_insert_of_not_mem heI]
 
-theorem er_eq_of_er_insert_le_forall (hXY : X ⊆ Y) (hY : ∀ e ∈ Y \ X, M.er (insert e X) ≤ M.er X) :
+lemma er_eq_of_er_insert_le_forall (hXY : X ⊆ Y) (hY : ∀ e ∈ Y \ X, M.er (insert e X) ≤ M.er X) :
     M.er X = M.er Y := by
   refine (M.er_mono hXY).eq_of_not_lt (fun hlt ↦ ?_)
   obtain ⟨e, he, hins⟩ := er_augment hlt
@@ -295,7 +295,7 @@ theorem er_eq_of_er_insert_le_forall (hXY : X ⊆ Y) (hY : ∀ e ∈ Y \ X, M.er
     WithTop.add_le_add_iff_left (fun htop ↦ not_top_lt (htop ▸ hlt))] at hY
   simp at hY
 
-theorem spanning_iff_er' [FiniteRk M] : M.Spanning X ↔ M.erk ≤ M.er X ∧ X ⊆ M.E := by
+lemma spanning_iff_er' [FiniteRk M] : M.Spanning X ↔ M.erk ≤ M.er X ∧ X ⊆ M.E := by
   refine' ⟨fun h ↦ _, fun ⟨hr, hX⟩ ↦ _⟩
   · rw [erk_eq_er_ground, ← er_cl_eq _ X, h.cl_eq]; exact ⟨rfl.le, h.subset_ground⟩
   obtain ⟨J, hJ⟩ := M.exists_basis X
@@ -305,39 +305,42 @@ theorem spanning_iff_er' [FiniteRk M] : M.Spanning X ↔ M.erk ≤ M.er X ∧ X 
   rw [spanning_iff_superset_base]
   exact ⟨J, hB, hJ.subset⟩
 
-theorem spanning_iff_er [FiniteRk M] (hX : X ⊆ M.E := by aesop_mat) :
+lemma spanning_iff_er [FiniteRk M] (hX : X ⊆ M.E := by aesop_mat) :
     M.Spanning X ↔ M.erk ≤ M.er X := by
   rw [spanning_iff_er', and_iff_left hX]
 
-theorem Spanning.er_eq (hX : M.Spanning X) : M.er X = M.erk := by
+lemma Spanning.er_eq (hX : M.Spanning X) : M.er X = M.erk := by
   obtain ⟨B, hB, hBX⟩ := hX.exists_base_subset
   rw [le_antisymm_iff, and_iff_right (M.er_le_erk _), ← hB.er]
   exact M.er_mono hBX
 
-theorem Loop.er_eq (he : M.Loop e) : M.er {e} = 0 := by
+lemma Loop.er_eq (he : M.Loop e) : M.er {e} = 0 := by
   rw [← er_cl_eq, he.cl, er_cl_eq, er_empty]
 
-theorem Nonloop.er_eq (he : M.Nonloop e) : M.er {e} = 1 := by
+lemma Nonloop.er_eq (he : M.Nonloop e) : M.er {e} = 1 := by
   rw [← he.indep.basis_self.encard, encard_singleton]
 
-theorem er_singleton_eq [Loopless M] (he : e ∈ M.E := by aesop_mat) :
+lemma er_singleton_eq [Loopless M] (he : e ∈ M.E := by aesop_mat) :
     M.er {e} = 1 :=
   (M.toNonloop he).er_eq
 
-theorem LoopEquiv.er_eq_er (h : M.LoopEquiv X Y) : M.er X = M.er Y := by
+lemma LoopEquiv.er_eq_er (h : M.LoopEquiv X Y) : M.er X = M.er Y := by
   rw [← M.er_cl_eq, h.cl_eq_cl, M.er_cl_eq]
 
-theorem er_eq_zero_iff (hX : X ⊆ M.E := by aesop_mat) :
+lemma er_eq_zero_iff (hX : X ⊆ M.E := by aesop_mat) :
     M.er X = 0 ↔ X ⊆ M.cl ∅ := by
   obtain ⟨I, hI⟩ := M.exists_basis X
   rw [← hI.encard, encard_eq_zero]
   exact ⟨by rintro rfl; exact hI.subset_cl, fun h ↦ eq_empty_of_forall_not_mem
     fun x hx ↦ (hI.indep.nonloop_of_mem hx).not_loop (h (hI.subset hx))⟩
 
-theorem er_eq_zero_iff' : M.er X = 0 ↔ X ∩ M.E ⊆ M.cl ∅ := by
+lemma er_eq_zero_iff' : M.er X = 0 ↔ X ∩ M.E ⊆ M.cl ∅ := by
   rw [← er_inter_ground_eq, er_eq_zero_iff]
 
-theorem er_eq_one_iff (hX : X ⊆ M.E := by aesop_mat) :
+@[simp] lemma er_loops (M : Matroid α) : M.er (M.cl ∅) = 0 := by
+  rw [er_eq_zero_iff]
+
+lemma er_eq_one_iff (hX : X ⊆ M.E := by aesop_mat) :
     M.er X = 1 ↔ ∃ e ∈ X, M.Nonloop e ∧ X ⊆ M.cl {e} := by
   refine ⟨?_, fun ⟨e, heX, he, hXe⟩ ↦ ?_⟩
   · obtain ⟨I, hI⟩ := M.exists_basis X
@@ -347,7 +350,7 @@ theorem er_eq_one_iff (hX : X ⊆ M.E := by aesop_mat) :
   rw [← he.er_eq]
   exact ((M.er_mono hXe).trans (M.er_cl_eq _).le).antisymm (M.er_mono (singleton_subset_iff.2 heX))
 
-theorem er_le_one_iff [M.Nonempty] (hX : X ⊆ M.E := by aesop_mat) :
+lemma er_le_one_iff [M.Nonempty] (hX : X ⊆ M.E := by aesop_mat) :
     M.er X ≤ 1 ↔ ∃ e ∈ M.E, X ⊆ M.cl {e} := by
   refine' ⟨fun h ↦ _, fun ⟨e, _, he⟩ ↦ _⟩
   · obtain ⟨I, hI⟩ := M.exists_basis X
@@ -372,160 +375,160 @@ section rFin
 def rFin (M : Matroid α) (X : Set α) :=
   M.er X < ⊤
 
-@[simp] theorem er_lt_top_iff : M.er X < ⊤ ↔ M.rFin X := Iff.rfl
+@[simp] lemma er_lt_top_iff : M.er X < ⊤ ↔ M.rFin X := Iff.rfl
 
-@[simp] theorem er_ne_top_iff : M.er X ≠ ⊤ ↔ M.rFin X :=
+@[simp] lemma er_ne_top_iff : M.er X ≠ ⊤ ↔ M.rFin X :=
   by rw [rFin, ← lt_top_iff_ne_top]
 
-theorem rFin.ne (h : M.rFin X) : M.er X ≠ ⊤ :=
+lemma rFin.ne (h : M.rFin X) : M.er X ≠ ⊤ :=
   er_ne_top_iff.2 h
 
-theorem rFin.lt (h : M.rFin X) : M.er X < ⊤ :=
+lemma rFin.lt (h : M.rFin X) : M.er X < ⊤ :=
   h
 
-theorem er_eq_top_iff : M.er X = ⊤ ↔ ¬M.rFin X := by rw [← er_ne_top_iff, not_ne_iff]
+lemma er_eq_top_iff : M.er X = ⊤ ↔ ¬M.rFin X := by rw [← er_ne_top_iff, not_ne_iff]
 
-@[simp] theorem rFin_inter_ground_iff : M.rFin (X ∩ M.E) ↔ M.rFin X := by
+@[simp] lemma rFin_inter_ground_iff : M.rFin (X ∩ M.E) ↔ M.rFin X := by
   rw [rFin, er_inter_ground_eq, rFin]
 
-theorem rFin.to_inter_ground (h : M.rFin X) : M.rFin (X ∩ M.E) :=
+lemma rFin.to_inter_ground (h : M.rFin X) : M.rFin (X ∩ M.E) :=
   rFin_inter_ground_iff.2 h
 
-theorem rFin.finite_of_basis' (h : M.rFin X) (hI : M.Basis' I X) : I.Finite := by
+lemma rFin.finite_of_basis' (h : M.rFin X) (hI : M.Basis' I X) : I.Finite := by
   rwa [← encard_lt_top_iff, hI.encard]
 
-theorem rFin.finite_of_basis (h : M.rFin X) (hI : M.Basis I X) : I.Finite := by
+lemma rFin.finite_of_basis (h : M.rFin X) (hI : M.Basis I X) : I.Finite := by
   rwa [← encard_lt_top_iff, hI.encard]
 
-theorem Basis'.finite_of_rFin (hI : M.Basis' I X) (h : M.rFin X) : I.Finite :=
+lemma Basis'.finite_of_rFin (hI : M.Basis' I X) (h : M.rFin X) : I.Finite :=
   h.finite_of_basis' hI
 
-theorem Basis.finite_of_rFin (hI : M.Basis I X) (h : M.rFin X) : I.Finite :=
+lemma Basis.finite_of_rFin (hI : M.Basis I X) (h : M.rFin X) : I.Finite :=
   h.finite_of_basis hI
 
-theorem rFin_iff' : M.rFin X ↔ ∃ I, M.Basis' I X ∧ I.Finite :=
+lemma rFin_iff' : M.rFin X ↔ ∃ I, M.Basis' I X ∧ I.Finite :=
   ⟨fun h ↦ (M.exists_basis' X).elim (fun I hI ↦ ⟨I, hI, h.finite_of_basis' hI⟩),
     fun ⟨I, hI, hIfin⟩ ↦ by rwa [← er_lt_top_iff, hI.er_eq_encard, encard_lt_top_iff]⟩
 
-theorem rFin_iff (hX : X ⊆ M.E := by aesop_mat) : M.rFin X ↔ ∃ I, M.Basis I X ∧ I.Finite := by
+lemma rFin_iff (hX : X ⊆ M.E := by aesop_mat) : M.rFin X ↔ ∃ I, M.Basis I X ∧ I.Finite := by
   simp_rw [rFin_iff', M.basis'_iff_basis hX]
 
-theorem rFin.exists_finite_basis' (h : M.rFin X) : ∃ I, M.Basis' I X ∧ I.Finite :=
+lemma rFin.exists_finite_basis' (h : M.rFin X) : ∃ I, M.Basis' I X ∧ I.Finite :=
   rFin_iff'.1 h
 
-theorem rFin.exists_finite_basis (h : M.rFin X) (hX : X ⊆ M.E := by aesop_mat) :
+lemma rFin.exists_finite_basis (h : M.rFin X) (hX : X ⊆ M.E := by aesop_mat) :
     ∃ I, M.Basis I X ∧ I.Finite :=
   (rFin_iff hX).1 h
 
-theorem Basis'.rFin_of_finite (hIX : M.Basis' I X) (h : I.Finite) : M.rFin X := by
+lemma Basis'.rFin_of_finite (hIX : M.Basis' I X) (h : I.Finite) : M.rFin X := by
   rwa [← er_ne_top_iff, ← hIX.encard, encard_ne_top_iff]
 
-theorem Basis'.rFin_iff_finite (hIX : M.Basis' I X) : M.rFin X ↔ I.Finite :=
+lemma Basis'.rFin_iff_finite (hIX : M.Basis' I X) : M.rFin X ↔ I.Finite :=
   ⟨hIX.finite_of_rFin, hIX.rFin_of_finite⟩
 
-theorem Basis.rFin_of_finite (hIX : M.Basis I X) (h : I.Finite) : M.rFin X := by
+lemma Basis.rFin_of_finite (hIX : M.Basis I X) (h : I.Finite) : M.rFin X := by
   rwa [← er_ne_top_iff, ← hIX.encard, encard_ne_top_iff]
 
-theorem Basis.rFin_iff_finite (hIX : M.Basis I X) : M.rFin X ↔ I.Finite :=
+lemma Basis.rFin_iff_finite (hIX : M.Basis I X) : M.rFin X ↔ I.Finite :=
   ⟨hIX.finite_of_rFin, hIX.rFin_of_finite⟩
 
-theorem Indep.rFin_iff_finite (hI : M.Indep I) : M.rFin I ↔ I.Finite :=
+lemma Indep.rFin_iff_finite (hI : M.Indep I) : M.rFin I ↔ I.Finite :=
   hI.basis_self.rFin_iff_finite
 
-theorem Indep.finite_of_rFin (hI : M.Indep I) (hfin : M.rFin I) : I.Finite :=
+lemma Indep.finite_of_rFin (hI : M.Indep I) (hfin : M.rFin I) : I.Finite :=
   hI.basis_self.finite_of_rFin hfin
 
-theorem rFin_of_finite (M : Matroid α) (hX : X.Finite) : M.rFin X :=
+lemma rFin_of_finite (M : Matroid α) (hX : X.Finite) : M.rFin X :=
   (M.er_le_encard X).trans_lt (encard_lt_top_iff.mpr hX)
 
-theorem Indep.subset_finite_basis'_of_subset_of_rFin (hI : M.Indep I) (hIX : I ⊆ X)
+lemma Indep.subset_finite_basis'_of_subset_of_rFin (hI : M.Indep I) (hIX : I ⊆ X)
     (hX : M.rFin X) : ∃ J, M.Basis' J X ∧ I ⊆ J ∧ J.Finite :=
   (hI.subset_basis'_of_subset hIX).imp fun _ hJ => ⟨hJ.1, hJ.2, hJ.1.finite_of_rFin hX⟩
 
-theorem Indep.subset_finite_basis_of_subset_of_rFin (hI : M.Indep I) (hIX : I ⊆ X)
+lemma Indep.subset_finite_basis_of_subset_of_rFin (hI : M.Indep I) (hIX : I ⊆ X)
     (hX : M.rFin X) (hXE : X ⊆ M.E := by aesop_mat) : ∃ J, M.Basis J X ∧ I ⊆ J ∧ J.Finite :=
   (hI.subset_basis_of_subset hIX).imp fun _ hJ => ⟨hJ.1, hJ.2, hJ.1.finite_of_rFin hX⟩
 
-theorem rFin_singleton (M : Matroid α) (e : α) : M.rFin {e} :=
+lemma rFin_singleton (M : Matroid α) (e : α) : M.rFin {e} :=
   M.rFin_of_finite (finite_singleton e)
 
-@[simp] theorem rFin_empty (M : Matroid α) : M.rFin ∅ :=
+@[simp] lemma rFin_empty (M : Matroid α) : M.rFin ∅ :=
   M.rFin_of_finite finite_empty
 
-theorem rFin.subset (h : M.rFin Y) (hXY : X ⊆ Y) : M.rFin X :=
+lemma rFin.subset (h : M.rFin Y) (hXY : X ⊆ Y) : M.rFin X :=
   (M.er_mono hXY).trans_lt h
 
-theorem not_rFin_superset (h : ¬M.rFin X) (hXY : X ⊆ Y) : ¬M.rFin Y :=
+lemma not_rFin_superset (h : ¬M.rFin X) (hXY : X ⊆ Y) : ¬M.rFin Y :=
   fun h' ↦ h (h'.subset hXY)
 
-theorem not_rFin_of_er_ge (h : ¬M.rFin X) (hXY : M.er X ≤ M.er Y) : ¬M.rFin Y :=
+lemma not_rFin_of_er_ge (h : ¬M.rFin X) (hXY : M.er X ≤ M.er Y) : ¬M.rFin Y :=
   fun h' ↦ h (hXY.trans_lt h')
 
-theorem rFin.finite_of_indep_subset (hX : M.rFin X) (hI : M.Indep I) (hIX : I ⊆ X) : I.Finite :=
+lemma rFin.finite_of_indep_subset (hX : M.rFin X) (hI : M.Indep I) (hIX : I ⊆ X) : I.Finite :=
   hI.finite_of_rFin (hX.to_inter_ground.subset (subset_inter hIX hI.subset_ground))
 
-@[simp] theorem rFin_ground_iff_finiteRk : M.rFin M.E ↔ M.FiniteRk := by
+@[simp] lemma rFin_ground_iff_finiteRk : M.rFin M.E ↔ M.FiniteRk := by
   obtain ⟨B, hB⟩ := M.exists_base
   use fun h => ⟨⟨B, hB, h.finite_of_indep_subset hB.indep hB.subset_ground⟩⟩
   simp_rw [rFin_iff (rfl.subset), basis_ground_iff]
   exact fun ⟨h⟩ ↦ h
 
-theorem rFin_ground (M : Matroid α) [FiniteRk M] : M.rFin M.E := by
+lemma rFin_ground (M : Matroid α) [FiniteRk M] : M.rFin M.E := by
   rwa [rFin_ground_iff_finiteRk]
 
-theorem erk_lt_top (M : Matroid α) [FiniteRk M] : M.erk < ⊤ := by
+lemma erk_lt_top (M : Matroid α) [FiniteRk M] : M.erk < ⊤ := by
   rw [erk_eq_er_ground, er_lt_top_iff]; exact M.rFin_ground
 
-theorem Indep.finite_of_subset_rFin (hI : M.Indep I) (hIX : I ⊆ X) (hX : M.rFin X) : I.Finite :=
+lemma Indep.finite_of_subset_rFin (hI : M.Indep I) (hIX : I ⊆ X) (hX : M.rFin X) : I.Finite :=
   hX.finite_of_indep_subset hI hIX
 
-theorem rFin.indep_of_encard_le_er (hX : M.rFin I) (h : encard I ≤ M.er I) : M.Indep I := by
+lemma rFin.indep_of_encard_le_er (hX : M.rFin I) (h : encard I ≤ M.er I) : M.Indep I := by
   rw [indep_iff_er_eq_encard_of_finite _]
   · exact (M.er_le_encard I).antisymm h
   simpa using h.trans_lt hX.lt
 
-theorem rFin.to_cl (h : M.rFin X) : M.rFin (M.cl X) := by
+lemma rFin.to_cl (h : M.rFin X) : M.rFin (M.cl X) := by
   rwa [← er_lt_top_iff, er_cl_eq]
 
-@[simp] theorem rFin_cl_iff : M.rFin (M.cl X) ↔ M.rFin X := by
+@[simp] lemma rFin_cl_iff : M.rFin (M.cl X) ↔ M.rFin X := by
   rw [← er_ne_top_iff, er_cl_eq, er_ne_top_iff]
 
-theorem rFin.union (hX : M.rFin X) (hY : M.rFin Y) : M.rFin (X ∪ Y) := by
+lemma rFin.union (hX : M.rFin X) (hY : M.rFin Y) : M.rFin (X ∪ Y) := by
   rw [← er_lt_top_iff] at *
   apply (M.er_union_le_er_add_er X Y).trans_lt
   rw [WithTop.add_lt_top]
   exact ⟨hX, hY⟩
 
-theorem rFin.rFin_union_iff (hX : M.rFin X) : M.rFin (X ∪ Y) ↔ M.rFin Y :=
+lemma rFin.rFin_union_iff (hX : M.rFin X) : M.rFin (X ∪ Y) ↔ M.rFin Y :=
   ⟨fun h ↦ h.subset subset_union_right, fun h ↦ hX.union h⟩
 
-theorem rFin.rFin_diff_iff (hX : M.rFin X) : M.rFin (Y \ X) ↔ M.rFin Y := by
+lemma rFin.rFin_diff_iff (hX : M.rFin X) : M.rFin (Y \ X) ↔ M.rFin Y := by
   rw [← hX.rFin_union_iff, union_diff_self, hX.rFin_union_iff]
 
-theorem rFin.inter_right (hX : M.rFin X) (Y : Set α) : M.rFin (X ∩ Y) :=
+lemma rFin.inter_right (hX : M.rFin X) (Y : Set α) : M.rFin (X ∩ Y) :=
   hX.subset inter_subset_left
 
-theorem rFin.inter_left (hX : M.rFin X) (Y : Set α) : M.rFin (Y ∩ X) :=
+lemma rFin.inter_left (hX : M.rFin X) (Y : Set α) : M.rFin (Y ∩ X) :=
   hX.subset inter_subset_right
 
-theorem rFin.diff (hX : M.rFin X) (D : Set α) : M.rFin (X \ D) :=
+lemma rFin.diff (hX : M.rFin X) (D : Set α) : M.rFin (X \ D) :=
   hX.subset diff_subset
 
-theorem rFin.insert (hX : M.rFin X) (e : α) : M.rFin (insert e X) := by
+lemma rFin.insert (hX : M.rFin X) (e : α) : M.rFin (insert e X) := by
   rw [← union_singleton]; exact hX.union (M.rFin_singleton e)
 
-@[simp] theorem rFin_insert_iff : M.rFin (insert e X) ↔ M.rFin X := by
+@[simp] lemma rFin_insert_iff : M.rFin (insert e X) ↔ M.rFin X := by
   rw [← singleton_union, (M.rFin_singleton e).rFin_union_iff]
 
-@[simp] theorem rFin_diff_singleton_iff : M.rFin (X \ {e}) ↔ M.rFin X := by
+@[simp] lemma rFin_diff_singleton_iff : M.rFin (X \ {e}) ↔ M.rFin X := by
   rw [(M.rFin_singleton e).rFin_diff_iff]
 
-theorem to_rFin (M : Matroid α) [FiniteRk M] (X : Set α) : M.rFin X := by
+lemma to_rFin (M : Matroid α) [FiniteRk M] (X : Set α) : M.rFin X := by
   obtain ⟨I, hI⟩ := M.exists_basis' X
   rw [← er_lt_top_iff, hI.er_eq_encard, encard_lt_top_iff]
   exact hI.indep.finite_of_subset_rFin hI.indep.subset_ground M.rFin_ground
 
-theorem rFin.cl_eq_cl_of_subset_of_er_ge_er (hX : M.rFin X) (hXY : X ⊆ Y) (hr : M.er Y ≤ M.er X) :
+lemma rFin.cl_eq_cl_of_subset_of_er_ge_er (hX : M.rFin X) (hXY : X ⊆ Y) (hr : M.er Y ≤ M.er X) :
     M.cl X = M.cl Y := by
   obtain ⟨I, hI⟩ := M.exists_basis' X
   obtain ⟨J, hJ, hIJ⟩ := hI.indep.subset_basis'_of_subset (hI.subset.trans hXY)
@@ -534,7 +537,7 @@ theorem rFin.cl_eq_cl_of_subset_of_er_ge_er (hX : M.rFin X) (hXY : X ⊆ Y) (hr 
     ← hJ.basis_inter_ground.cl_eq_cl, Finite.eq_of_subset_of_encard_le'
       (hI.indep.finite_of_subset_rFin hI.subset hX) hIJ hr]
 
-theorem er_union_eq_of_subset_of_er_le_er (Z : Set α) (hXY : X ⊆ Y) (hr : M.er Y ≤ M.er X) :
+lemma er_union_eq_of_subset_of_er_le_er (Z : Set α) (hXY : X ⊆ Y) (hr : M.er Y ≤ M.er X) :
     M.er (X ∪ Z) = M.er (Y ∪ Z) := by
   obtain hX' | hX' := em (M.rFin X)
   · rw [← er_union_cl_left_eq, hX'.cl_eq_cl_of_subset_of_er_ge_er hXY hr, er_union_cl_left_eq]
@@ -542,12 +545,12 @@ theorem er_union_eq_of_subset_of_er_le_er (Z : Set α) (hXY : X ⊆ Y) (hr : M.e
   · exact not_rFin_of_er_ge hX' (M.er_mono (subset_union_of_subset_left hXY _))
   exact not_rFin_of_er_ge hX' (M.er_mono subset_union_left)
 
-theorem er_union_eq_of_subsets_of_ers_le (hX : X ⊆ X') (hY : Y ⊆ Y') (hXX' : M.er X' ≤ M.er X)
+lemma er_union_eq_of_subsets_of_ers_le (hX : X ⊆ X') (hY : Y ⊆ Y') (hXX' : M.er X' ≤ M.er X)
     (hYY' : M.er Y' ≤ M.er Y) : M.er (X ∪ Y) = M.er (X' ∪ Y') := by
   rw [er_union_eq_of_subset_of_er_le_er _ hX hXX', union_comm,
     er_union_eq_of_subset_of_er_le_er _ hY hYY', union_comm]
 
-theorem rFin.basis_of_subset_cl_of_subset_of_encard_le (hX : M.rFin X) (hXI : X ⊆ M.cl I)
+lemma rFin.basis_of_subset_cl_of_subset_of_encard_le (hX : M.rFin X) (hXI : X ⊆ M.cl I)
     (hIX : I ⊆ X) (hI : I.encard ≤ M.er X) : M.Basis I X := by
   obtain ⟨J, hJ⟩ := M.exists_basis (I ∩ M.E)
   have hIJ := hJ.subset.trans inter_subset_left
@@ -557,7 +560,7 @@ theorem rFin.basis_of_subset_cl_of_subset_of_encard_le (hX : M.rFin X) (hXI : X 
   rw [← hJX.encard] at hI
   rwa [← Finite.eq_of_subset_of_encard_le' (hX.finite_of_basis hJX) hIJ hI]
 
-theorem rFin.iUnion [Fintype ι] {Xs : ι → Set α} (h : ∀ i, M.rFin (Xs i)) : M.rFin (⋃ i, Xs i) := by
+lemma rFin.iUnion [Fintype ι] {Xs : ι → Set α} (h : ∀ i, M.rFin (Xs i)) : M.rFin (⋃ i, Xs i) := by
   choose Is hIs using fun i ↦ M.exists_basis' (Xs i)
   have hfin : (⋃ i, Is i).Finite := finite_iUnion <| fun i ↦ (h i).finite_of_basis' (hIs i)
   rw [← rFin_cl_iff]
@@ -579,98 +582,127 @@ noncomputable def r (M : Matroid α) (X : Set α) : ℕ :=
 @[reducible] noncomputable def rk (M : Matroid α) : ℕ :=
   ENat.toNat M.erk
 
-theorem rk_def (M : Matroid α) : M.rk = M.r M.E := by
+lemma rk_def (M : Matroid α) : M.rk = M.r M.E := by
   rw [rk,r,er,restrict_ground_eq_self]
 
-@[simp] theorem er_toNat_eq_r (M : Matroid α) (X : Set α) : ENat.toNat (M.er X) = M.r X :=
+@[simp] lemma er_toNat_eq_r (M : Matroid α) (X : Set α) : ENat.toNat (M.er X) = M.r X :=
   rfl
 
-theorem Base.ncard (hB : M.Base B) : B.ncard = M.rk := by
+lemma Base.ncard (hB : M.Base B) : B.ncard = M.rk := by
   rw [rk_def, ← er_toNat_eq_r, ncard_def, hB.encard, erk_eq_er_ground]
 
-theorem rFin.coe_r_eq (hX : M.rFin X) : (M.r X : ℕ∞) = M.er X := by
+lemma rFin.coe_r_eq (hX : M.rFin X) : (M.r X : ℕ∞) = M.er X := by
   rw [r, coe_toNat (by rwa [er_ne_top_iff])]
 
-theorem coe_r_eq_er_of_finite (M : Matroid α) (hX : X.Finite) : (M.r X : ℕ∞) = M.er X :=
+lemma coe_r_eq_er_of_finite (M : Matroid α) (hX : X.Finite) : (M.r X : ℕ∞) = M.er X :=
   (M.rFin_of_finite hX).coe_r_eq
 
-@[simp] theorem coe_r_eq (M : Matroid α) [FiniteRk M] (X : Set α) : (M.r X : ℕ∞) = M.er X :=
+@[simp] lemma coe_r_eq (M : Matroid α) [FiniteRk M] (X : Set α) : (M.r X : ℕ∞) = M.er X :=
   (M.to_rFin X).coe_r_eq
 
-theorem r_eq_of_er_eq (h : M.er X = M.er Y) : M.r X = M.r Y := by
+lemma r_eq_of_er_eq (h : M.er X = M.er Y) : M.r X = M.r Y := by
   rw [r, r, h]
 
-theorem rFin.er_eq_er_iff (hX : M.rFin X) (hY : M.rFin Y) : M.er X = M.er Y ↔ M.r X = M.r Y := by
+lemma rFin.er_eq_er_iff (hX : M.rFin X) (hY : M.rFin Y) : M.er X = M.er Y ↔ M.r X = M.r Y := by
   rw [← hX.coe_r_eq, ← hY.coe_r_eq, Nat.cast_inj]
 
-theorem rFin.er_le_er_iff (hX : M.rFin X) (hY : M.rFin Y) : M.er X ≤ M.er Y ↔ M.r X ≤ M.r Y := by
+lemma rFin.er_le_er_iff (hX : M.rFin X) (hY : M.rFin Y) : M.er X ≤ M.er Y ↔ M.r X ≤ M.r Y := by
   rw [← hX.coe_r_eq, ← hY.coe_r_eq, Nat.cast_le]
 
-@[simp] theorem er_eq_er_iff [FiniteRk M] : M.er X = M.er Y ↔ M.r X = M.r Y :=
+@[simp] lemma er_eq_er_iff [FiniteRk M] : M.er X = M.er Y ↔ M.r X = M.r Y :=
   (M.to_rFin X).er_eq_er_iff (M.to_rFin Y)
 
-@[simp] theorem er_le_er_iff [FiniteRk M] : M.er X ≤ M.er Y ↔ M.r X ≤ M.r Y := by
+@[simp] lemma er_le_er_iff [FiniteRk M] : M.er X ≤ M.er Y ↔ M.r X ≤ M.r Y := by
   rw [← coe_r_eq, ← coe_r_eq, Nat.cast_le]
 
-@[simp] theorem er_eq_coe_iff [FiniteRk M] {n : ℕ} : M.er X = n ↔ M.r X = n := by
+@[simp] lemma er_eq_coe_iff [FiniteRk M] {n : ℕ} : M.er X = n ↔ M.r X = n := by
   rw [← coe_r_eq, Nat.cast_inj]
 
-@[simp] theorem er_le_coe_iff [FiniteRk M] {n : ℕ} : M.er X ≤ n ↔ M.r X ≤ n := by
+@[simp] lemma er_le_coe_iff [FiniteRk M] {n : ℕ} : M.er X ≤ n ↔ M.r X ≤ n := by
   rw [← coe_r_eq, Nat.cast_le]
 
-@[simp] theorem coe_le_er_iff [FiniteRk M] {n : ℕ} : (n : ℕ∞) ≤ M.er X ↔ n ≤ M.r X := by
+@[simp] lemma coe_le_er_iff [FiniteRk M] {n : ℕ} : (n : ℕ∞) ≤ M.er X ↔ n ≤ M.r X := by
   rw [← coe_r_eq, Nat.cast_le]
 
-theorem rFin.r_le_r_of_er_le_er (hY : M.rFin Y) (hle : M.er X ≤ M.er Y) : M.r X ≤ M.r Y := by
+lemma rFin.r_le_r_of_er_le_er (hY : M.rFin Y) (hle : M.er X ≤ M.er Y) : M.r X ≤ M.r Y := by
   rwa [← rFin.er_le_er_iff _ hY]; exact hle.trans_lt hY.lt
 
-theorem r_eq_r_inter_ground (M : Matroid α) (X : Set α) : M.r X = M.r (X ∩ M.E) := by
+lemma r_eq_r_inter_ground (M : Matroid α) (X : Set α) : M.r X = M.r (X ∩ M.E) := by
   rw [← er_toNat_eq_r, ← er_inter_ground_eq, er_toNat_eq_r]
 
-theorem le_r_iff [FiniteRk M] {n : ℕ} : n ≤ M.r X ↔ ∃ I, I ⊆ X ∧ M.Indep I ∧ I.ncard = n := by
+lemma le_r_iff [FiniteRk M] {n : ℕ} : n ≤ M.r X ↔ ∃ I, I ⊆ X ∧ M.Indep I ∧ I.ncard = n := by
   simp_rw [← coe_le_er_iff, le_er_iff,]
   refine ⟨fun ⟨I, hIX, hI, hc⟩ ↦ ⟨I, hIX, hI, by rw [ncard_def, hc, toNat_coe]⟩,
     fun ⟨I, hIX, hI, hc⟩ ↦ ⟨I, hIX, hI, ?_⟩⟩
   rw [hI.finite.encard_eq_coe, ← hc]; rfl
 
-theorem r_le_iff [FiniteRk M] {n : ℕ} : M.r X ≤ n ↔ ∀ {I}, I ⊆ X → M.Indep I → I.ncard ≤ n := by
+lemma r_le_iff [FiniteRk M] {n : ℕ} : M.r X ≤ n ↔ ∀ {I}, I ⊆ X → M.Indep I → I.ncard ≤ n := by
   simp_rw [← er_le_coe_iff, er_le_iff, encard_le_coe_iff]
   refine ⟨fun h I hIX hI ↦ ?_, fun h I hIX hI ↦ ⟨hI.finite, ⟨_, hI.finite.encard_eq_coe, h hIX hI⟩⟩⟩
   obtain ⟨-, m, hm, hmn⟩ := h hIX hI
   rwa [ncard_def, hm, toNat_coe]
 
-theorem r_mono (M : Matroid α) [FiniteRk M] : Monotone M.r := by
+lemma r_mono (M : Matroid α) [FiniteRk M] : Monotone M.r := by
   rintro X Y (hXY : X ⊆ Y);
   rw [← er_le_er_iff]
   exact M.er_mono hXY
 
-theorem r_le_rk (M : Matroid α) [FiniteRk M] (X : Set α) : M.r X ≤ M.rk := by
+lemma r_le_rk (M : Matroid α) [FiniteRk M] (X : Set α) : M.r X ≤ M.rk := by
   rw [r_eq_r_inter_ground, rk_def]; exact M.r_mono inter_subset_right
 
-theorem Indep.r (hI : M.Indep I) : M.r I = I.ncard := by
+lemma Indep.r (hI : M.Indep I) : M.r I = I.ncard := by
   rw [← er_toNat_eq_r, hI.er, ncard_def]
 
-theorem r_le_card (M : Matroid α) [Matroid.Finite M] (X : Set α) (hX : X ⊆ M.E := by aesop_mat) :
+lemma r_le_card (M : Matroid α) [Matroid.Finite M] (X : Set α) (hX : X ⊆ M.E := by aesop_mat) :
     M.r X ≤ X.ncard :=
   r_le_iff.2 <| fun {I} hI _ ↦ (ncard_le_ncard hI (M.set_finite X))
 
-theorem Indep.card_le_r_of_subset [FiniteRk M] (hI : M.Indep I) (h : I ⊆ X) : I.ncard ≤ M.r X := by
+lemma Indep.card_le_r_of_subset [FiniteRk M] (hI : M.Indep I) (h : I ⊆ X) : I.ncard ≤ M.r X := by
   rw [← hI.r]; exact M.r_mono h
 
-theorem Indep.card_le_rk [FiniteRk M] (hI : M.Indep I) : I.ncard ≤ M.rk :=
+lemma Indep.card_le_rk [FiniteRk M] (hI : M.Indep I) : I.ncard ≤ M.rk :=
   hI.r.symm.trans_le (M.r_le_rk I)
 
-theorem Basis'.card (h : M.Basis' I X) : I.ncard = M.r X := by
+lemma Basis'.card (h : M.Basis' I X) : I.ncard = M.r X := by
   rw [ncard_def, h.encard, ← er_toNat_eq_r]
 
-theorem Basis'.r (h : M.Basis' I X) : M.r I = M.r X := by
+lemma Basis'.r (h : M.Basis' I X) : M.r I = M.r X := by
   rw [← h.card, h.indep.r]
 
-theorem Basis.card (h : M.Basis I X) : I.ncard = M.r X :=
+lemma Basis.card (h : M.Basis I X) : I.ncard = M.r X :=
   h.basis'.card
 
-theorem Basis.r (h : M.Basis I X) : M.r I = M.r X :=
+lemma Basis.r (h : M.Basis I X) : M.r I = M.r X :=
   h.basis'.r
+
+lemma r_eq_zero_iff [FiniteRk M] (hX : X ⊆ M.E) : M.r X = 0 ↔ X ⊆ M.cl ∅ := by
+  rw [← er_eq_coe_iff, coe_zero, er_eq_zero_iff]
+
+@[simp] lemma r_loops (M : Matroid α) : M.r (M.cl ∅) = 0 := by
+  simp [r]
+
+lemma Nonloop.r_eq (he : M.Nonloop e) : M.r {e} = 1 := by
+  rw [r, he.er_eq]; rfl
+
+lemma Loop.r_eq (he : M.Loop e) : M.r {e} = 0 := by
+  rw [r, he.er_eq]; rfl
+
+lemma rFin.submod (hX : M.rFin X) (hY : M.rFin Y) : M.r (X ∩ Y) + M.r (X ∪ Y) ≤ M.r X + M.r Y := by
+  obtain ⟨c, h_eq⟩ := le_iff_exists_add.1 <| M.er_inter_add_er_union_le_er_add_er X Y
+  obtain (rfl | hc) := eq_or_ne c ⊤
+  · rw [add_top, WithTop.add_eq_top] at h_eq
+    simp [hX.ne, hY.ne] at h_eq
+  have hi : M.rFin (X ∩ Y) := hX.subset inter_subset_left
+  have hu : M.rFin (X ∪ Y) := hX.union hY
+  rw [← ge_iff_le, r,r, ge_iff_le, ← toNat_add hX.ne hY.ne, h_eq, toNat_add _ hc,
+    toNat_add hi.ne hu.ne, ← r, ← r]
+  · apply Nat.le_add_right
+  rw [Ne, WithTop.add_eq_top, not_or]
+  exact ⟨hi.ne, hu.ne⟩
+
+lemma r_submod (M : Matroid α) [FiniteRk M] (X Y : Set α) :
+    M.r (X ∩ Y) + M.r (X ∪ Y) ≤ M.r X + M.r Y :=
+  rFin.submod (M.to_rFin X) (M.to_rFin Y)
 
 end Rank
 
@@ -678,42 +710,42 @@ section Constructions
 
 variable {E : Set α}
 
-@[simp] theorem loopyOn_er_eq (E X : Set α) : (loopyOn E).er X = 0 := by
+@[simp] lemma loopyOn_er_eq (E X : Set α) : (loopyOn E).er X = 0 := by
   obtain ⟨I, hI⟩ := (loopyOn E).exists_basis' X
   rw [hI.er_eq_encard, loopyOn_indep_iff.1 hI.indep, encard_empty]
 
-@[simp] theorem loopyOn_erk_eq (E : Set α) : (loopyOn E).erk = 0 := by
+@[simp] lemma loopyOn_erk_eq (E : Set α) : (loopyOn E).erk = 0 := by
   rw [erk_eq_er_ground, loopyOn_er_eq]
 
-@[simp] theorem loopyOn_r_eq (E X : Set α) : (loopyOn E).r X = 0 := by
+@[simp] lemma loopyOn_r_eq (E X : Set α) : (loopyOn E).r X = 0 := by
   rw [← er_toNat_eq_r, loopyOn_er_eq]; rfl
 
-@[simp] theorem erk_eq_zero_iff : M.erk = 0 ↔ M = loopyOn M.E := by
+@[simp] lemma erk_eq_zero_iff : M.erk = 0 ↔ M = loopyOn M.E := by
   refine ⟨fun h ↦ cl_empty_eq_ground_iff.1 ?_, fun h ↦ by rw [h, loopyOn_erk_eq]⟩
   obtain ⟨B, hB⟩ := M.exists_base
   rw [← hB.encard, encard_eq_zero] at h
   rw [← h, hB.cl_eq]
 
-@[simp] theorem erk_loopyOn_eq_zero (α : Type*) : (emptyOn α).erk = 0 := by
+@[simp] lemma erk_loopyOn_eq_zero (α : Type*) : (emptyOn α).erk = 0 := by
   rw [erk_eq_zero_iff, emptyOn_ground, loopyOn_empty]
 
-theorem eq_loopyOn_iff_cl : M = loopyOn E ↔ M.cl ∅ = E ∧ M.E = E :=
+lemma eq_loopyOn_iff_cl : M = loopyOn E ↔ M.cl ∅ = E ∧ M.E = E :=
   ⟨fun h ↦ by rw [h]; simp, fun ⟨h,h'⟩ ↦ by rw [← h', ← cl_empty_eq_ground_iff, h, h']⟩
 
-theorem eq_loopyOn_iff_erk : M = loopyOn E ↔ M.erk = 0 ∧ M.E = E :=
+lemma eq_loopyOn_iff_erk : M = loopyOn E ↔ M.erk = 0 ∧ M.E = E :=
   ⟨fun h ↦ by rw [h]; simp, fun ⟨h,h'⟩ ↦ by rw [← h', ← erk_eq_zero_iff, h]⟩
 
-@[simp] theorem freeOn_erk_eq (E : Set α) : (freeOn E).erk = E.encard := by
+@[simp] lemma freeOn_erk_eq (E : Set α) : (freeOn E).erk = E.encard := by
   rw [erk_eq_er_ground, freeOn_ground, (freeOn_indep_iff.2 rfl.subset).er]
 
-theorem freeOn_er_eq (hXE : X ⊆ E) : (freeOn E).er X = X.encard := by
+lemma freeOn_er_eq (hXE : X ⊆ E) : (freeOn E).er X = X.encard := by
   obtain ⟨I, hI⟩ := (freeOn E).exists_basis X
   rw [hI.er_eq_encard, (freeOn_indep hXE).eq_of_basis hI]
 
-theorem freeOn_r_eq (hXE : X ⊆ E) : (freeOn E).r X = X.ncard := by
+lemma freeOn_r_eq (hXE : X ⊆ E) : (freeOn E).r X = X.ncard := by
   rw [← er_toNat_eq_r, freeOn_er_eq hXE, ncard_def]
 
--- theorem IsIso.erk_eq_erk {α β : Type*} {M : Matroid α} {N : Matroid β} (h : M ≂ N) :
+-- lemma IsIso.erk_eq_erk {α β : Type*} {M : Matroid α} {N : Matroid β} (h : M ≂ N) :
 --     M.erk = N.erk := by
 --   obtain (⟨rfl, rfl⟩ | ⟨⟨e⟩⟩) := h; simp; exact e.erk_eq_erk
 
